hip/hip_graphmark_proofs.v
@@ -5,6 +5,7 @@ Require Import VST.msl.seplog.
 Require Import VST.msl.log_normalize.
 Require Import RamifyCoq.lib.Coqlib.
 Require Import RamifyCoq.lib.EquivDec_ext.
+Require Import RamifyCoq.lib.Relation_ext.
 Require Import RamifyCoq.hip.hip_graphmark.
 Require Import RamifyCoq.msl_ext.seplog.
 Require Import RamifyCoq.graph.graph_model.
@@ -16,12 +17,15 @@ Require Import RamifyCoq.msl_application.Graph.
 Require Import RamifyCoq.msl_application.GraphBi.
 Require Import RamifyCoq.msl_application.Graph_Mark.
 Require Import RamifyCoq.msl_application.GraphBi_Mark.
+Import RamifyCoq.msl_ext.seplog.OconNotation.
 
 Context {pSGG_Bi: pSpatialGraph_Graph_Bi}.
 Context {sSGG_Bi: sSpatialGraph_Graph_Bi}.
 Context {SGSA: SpatialGraphStrongAssum SGP}.
 
 Tactic Notation "LEM" constr(v) := (destruct (classic v); auto).
+
+Axiom TT_prop_right_reverse: forall {A : Type} {ND : NatDed A} (P : Prop), TT |-- !!P -> P.
 
 Module GraphMark <: Mgraphmark.
   Definition formula : Type := pred.
@@ -51,186 +55,202 @@ Module GraphMark <: Mgraphmark.
 
   Lemma update_is_mark1: forall (l r: addr) (G G1: A) x,
       vvalid G x ->
-      step_list G x (l :: r :: nil) ->
-      valid (update G x true l r G1) ->
+      dst G (x, L) = l -> dst G (x, R) = r ->
+      (exists (Hn : ~ is_null G x) (Hi : graph_gen.in_math G x l r),
+          Graph_gen_update G x true l r Hi Hn = G1) ->
       mark1 x G G1.
   Proof.
-    intros. unfold valid in H1. 
-
-    destruct H1 as [Hi [Hn ?]]. rewrite <- H1. split. intro z. split. destruct (t_eq_dec z x); split; intro. hnf.
-    left; auto. hnf in H2. subst; auto. left; auto. hnf in H2. destruct H2. auto. exfalso; auto. simpl. unfold change_edge_func.
-    destruct (t_eq_dec z x). subst. rewrite H0. auto. auto. split. auto. split. hnf. simpl. unfold change_node_label.
-    destruct (@t_eq_dec adr natEqDec x x). auto. exfalso; auto. intros. simpl. unfold change_node_label.
-    destruct (t_eq_dec n' x). exfalso; auto. auto.
+    intros. unfold valid in H1. destruct H2 as [Hn [Hi ?]].
+    rewrite <- H2. split; [|split]; simpl.
+    + split; [|split; [|split]]; simpl; intros; auto.
+      - unfold graph_gen.change_vvalid. intuition. subst; auto.
+      - unfold graph_gen.change_evalid. intuition.
+        rewrite (@only_two_edges _ _ _ _ G _ _ (biGraph G)) in H4.
+        destruct H4; rewrite H3;
+        [apply (@left_valid _ _ _ _ _ _ _ (biGraph G)) |
+         apply (@right_valid _ _ _ _ _ _ _ (biGraph G))]; auto.
+      - unfold graph_gen.change_dst. destruct (equiv_dec (src G e) x); auto.
+        unfold equiv in e0.
+        destruct (left_or_right G (biGraph G) x e e0); subst e; auto.
+    + unfold graph_gen.update_vlabel. destruct (equiv_dec x x); intuition.
+    + intros. unfold graph_gen.update_vlabel. destruct (equiv_dec x n'); intuition.
   Qed.
 
-  Lemma node_is_two: forall (G : A) x l r,
-      @graph.valid adr nat natEqDec (b_pg_g G) x ->
-      @graph.valid adr nat natEqDec (b_pg_g G) l ->
-      @graph.valid adr nat natEqDec (b_pg_g G) r ->
-      @edge_func adr nat natEqDec (b_pg_g G) x = l :: r :: nil ->
-      node_connected_two adr nat natEqDec (b_pg_g G) x l r.
+  Lemma marked_node_marked: forall (G1: A) (n: addr) (G2: A) (x: addr) (v: bool),
+      vlabel G1 x = true ->
+      WeakMarkGraph.mark n G1 G2 ->
+      vlabel G2 x = true.
   Proof.
-    intros. split. do 2 (split; auto). rewrite H2. apply in_eq. split. do 2 (split; auto). rewrite H2. apply in_cons, in_eq.
-    intros. destruct H3 as [? [? ?]]. rewrite H2 in H5. apply in_inv in H5; destruct H5. left; auto. apply in_inv in H5.
-    destruct H5. right; auto. inversion H5.
-  Qed.
-
-  Lemma marked_node_marked: forall G1 n w G2 x, @node_label adr nat natEqDec (b_pg_g G1) x = 1 ->
-                                                mark G1 n G2 w ->
-                                                @node_label adr nat natEqDec (b_pg_g G2) x = 1.
-  Proof.
-    intros. destruct H0 as [? [? ?]]. LEM ((b_pg_g G1) |= n ~o~> x satisfying (unmarked nat (fun d : nat => d = 1))).
-    specialize (H1 _ H3). hnf in H1. auto. specialize (H2 _ H3). rewrite <- H2. auto.
-  Qed.
-
-  Lemma three_identity_same:
-    forall (G G1 G2 G3 : A) x l r, (b_pg_g G) ~=~ (b_pg_g G1) ->
-                                   (b_pg_g G1) ~=~ (b_pg_g G2) ->
-                                   (b_pg_g G2) ~=~ (b_pg_g G3) ->
-                                   @graph.valid adr nat natEqDec (b_pg_g G) x ->
-                                   @graph.valid adr nat natEqDec (b_pg_g G) l ->
-                                   @graph.valid adr nat natEqDec (b_pg_g G) r ->
-                                   @edge_func adr nat natEqDec (b_pg_g G) x = l :: r :: nil ->
-                                   @graph.valid adr nat natEqDec (b_pg_g G3) x /\
-                                   @graph.valid adr nat natEqDec (b_pg_g G3) l /\
-                                   @graph.valid adr nat natEqDec (b_pg_g G3) r /\
-                                   @edge_func adr nat natEqDec (b_pg_g G3) x = l :: r :: nil.
-  Proof.
-    intros. assert ((b_pg_g G) ~=~ (b_pg_g G3)). apply (si_trans H). apply (si_trans H0). auto. split. destruct (H6 x).
-    rewrite <- H7; auto. split. destruct (H6 l). rewrite <- H7; auto. split. destruct (H6 r). rewrite <- H7; auto.
-    destruct (H6 x). rewrite <- H8; auto.
+    intros. unfold WeakMarkGraph.mark. destruct H0 as [? ?]. specialize (H1 x).
+    simpl in H1. symmetry. rewrite H1. left; auto.
   Qed.
   
-  Lemma axiom_1 : forall v G1 G2 G G3 x l r, valid (imp (and (lookup G x v l r) (and (mark G r G1) (and (neq v 1) (and (mark G2 l G3) (update G1 x 1 l r G2))))) (and (mark G x G3) (lookup G3 x 1 l r))).
+  Lemma axiom_6 : forall v G1 G2 G G3 x l r,
+      valid (imp (and (lookup G x v l r)
+                      (and (update G x true l r G1)
+                           (and (neq v true) (and (mark G1 l G2) (mark G2 r G3)))))
+                 (and (mark G x G3) (lookup G3 x true l r))).
   Proof.
-    intros; intro w; hnf; unfold and; hnf; intros. destruct H as [? [? [? [? ?]]]]. destruct H as [? [? [? [? ?]]]]. hnf in H1.
-    assert (mark1 adr nat natEqDec (fun d : nat => d = 1) (b_pg_g G1) x (b_pg_g G2)).
-    apply (update_is_mark1 l r w); auto; destruct H0 as [? _]; destruct (H0 x). tauto. rewrite <- H9. auto. split.
-    apply (mark_right_root_left _ _ _ _ _ (b_pg_g G1) (b_pg_g G2) _ _ l r); auto. hnf; simpl. rewrite H. auto.
-    apply node_is_two; auto. destruct H8 as [? [? [? ?]]]. split. hnf in H10. apply (marked_node_marked G2 l w); auto.
-    destruct H0, H2. apply (three_identity_same G G1 G2); auto.
+    intros. unfold valid, imp, and, lookup, neq, mark, update.
+    apply imp_andp_adjoint. normalize. destruct H as [? [? [? [? [? ?]]]]].
+    assert (mark1 x G G1) by (apply (update_is_mark1 l r); auto).
+    apply andp_right; normalize.
+    + destruct H0 as [Hn [Hi ?]].
+      apply mark1_mark_list_mark with (l :: r :: nil); auto.
+      - simpl. unfold Complement. unfold In. clear - H H1. subst v. intuition.
+      - apply gamma_step_list with false; auto. simpl. unfold gamma.
+        do 2 (f_equal; auto). subst v. apply Bool.not_true_is_false in H1. auto.
+      - hnf. apply (compond_intro (compond_relation Logic.eq (mark1 x)) _ _ G1 _).
+        apply (compond_intro Logic.eq (mark1 x) G G G1); auto.
+        unfold mark_list. simpl. hnf.
+        apply (compond_intro
+                 (compond_relation Logic.eq (Graph_Mark.mark l)) _ _ G2 _); auto.
+          apply (compond_intro Logic.eq (Graph_Mark.mark l) G1 G1 G2); auto.
+    + destruct H2, H3, H9. destruct H12 as [? ?]. split.
+      - apply (marked_node_marked G2 r); auto. apply (marked_node_marked G1 l); auto. 
+      - assert (G ~=~ G3) by (transitivity G1; auto; transitivity G2; auto).
+        destruct H14 as [? [? [? ?]]]. split; [|split; [|split; [|split]]].
+        * specialize (H14 x); intuition.
+        * specialize (H14 l); intuition.
+        * specialize (H14 r); intuition.
+        * assert (evalid G (x, L)) by
+              (apply (@left_valid _ _ _ _ _ _ _ (biGraph G)); auto).
+          subst l. symmetry. specialize (H17 (x, L)).
+          specialize (H15 (x, L)). intuition.
+        * assert (evalid G (x, R)) by
+              (apply (@right_valid _ _ _ _ _ _ _ (biGraph G)); auto).
+          subst r. symmetry. specialize (H17 (x, R)).
+          specialize (H15 (x, R)). intuition.
   Qed.
 
-  Lemma axiom_2 : forall v G1 G2 G G3 x l r, valid (imp (and (lookup G x v l r) (and (mark G l G1) (and (neq v 1) (and (mark G2 r G3) (update G1 x 1 l r G2))))) (and (mark G x G3) (lookup G3 x 1 l r))).
+  Lemma axiom_7 : forall v G x G1 y l r,
+      valid (imp (and (mark G x G1) (lookup G y v l r))
+                 (and (subset_reach G x G1)
+                      (and (eq_notreach G x G1)
+                           (ext (fun Anon_15 => (lookup G1 y Anon_15 l r)))))).
   Proof.
-    intros; intro w; hnf; unfold and; hnf; intros. destruct H as [? [? [? [? ?]]]]. destruct H as [? [? [? [? ?]]]]. hnf in H1.
-    assert (mark1 adr nat natEqDec (fun d : nat => d = 1) (b_pg_g G1) x (b_pg_g G2)).
-    apply (update_is_mark1 l r w); auto; destruct H0 as [? _]; destruct (H0 x). tauto. rewrite <- H9. auto. split.
-    apply (mark_left_root_right _ _ _ _ _ (b_pg_g G1) (b_pg_g G2) _ _ l r); auto. hnf; simpl. rewrite H. auto.
-    apply node_is_two; auto. destruct H8 as [? [? [? ?]]]. split. hnf in H10. apply (marked_node_marked G2 r w); auto.
-    destruct H0, H2. apply (three_identity_same G G1 G2); auto.
+    intros. unfold valid, imp, and, mark, lookup, subset_reach, eq_notreach.
+    apply imp_andp_adjoint. normalize. destruct H0 as [? [? [? [? [? ?]]]]].
+    apply andp_right; [|apply andp_right].
+    + apply TT_prop_right. destruct H. apply (reachable_ind.si_reachable _ _ x) in H6.
+      destruct H6. auto.
+    + apply TT_prop_right. destruct H. unfold unreachable_partialgraph.
+      apply partialgraph_proper; auto. hnf.
+      split; intro z; unfold In; rewrite H6; auto.
+    + unfold ext. destruct H as [[? ?] ?]. specialize (H6 y). simpl in H6.
+      destruct H7 as [? [? [? ?]]].
+      LEM (G |= x ~o~> y satisfying (WeakMarkGraph.unmarked G)).
+      - assert (vlabel G1 y = true) by (symmetry; rewrite H6; right; auto).
+        apply (exp_right true). normalize. split; [|split;[|split;[|split; [|split]]]]; auto.
+        * specialize (H7 y); intuition.
+        * specialize (H7 l); intuition.
+        * specialize (H7 r); intuition.
+        * assert (evalid G (y, L)) by
+              (apply (@left_valid _ _ _ _ _ _ _ (biGraph G)); auto).
+          subst l. symmetry. specialize (H10 (y, L)).
+          specialize (H8 (y, L)). intuition.
+        * assert (evalid G (y, R)) by
+              (apply (@right_valid _ _ _ _ _ _ _ (biGraph G)); auto).
+          subst r. symmetry. specialize (H10 (y, R)).
+          specialize (H8 (y, R)). intuition.
+      - apply (exp_right v). normalize. split; [|split;[|split;[|split; [|split]]]].
+        * destruct (Bool.bool_dec v true).
+          1: rewrite e in *; symmetry; rewrite H6; left; auto.
+          apply Bool.not_true_is_false in n. rewrite n in *. clear n.
+          apply Bool.not_true_is_false. intro. symmetry in H12. rewrite H6 in H12.
+          destruct H12; [|intuition]. apply Bool.diff_true_false. clear - H0 H12.
+          rewrite H12. rewrite <- H0. auto.
+        * specialize (H7 y); intuition.
+        * specialize (H7 l); intuition.
+        * specialize (H7 r); intuition.
+        * assert (evalid G (y, L)) by
+              (apply (@left_valid _ _ _ _ _ _ _ (biGraph G)); auto).
+          subst l. symmetry. specialize (H10 (y, L)).
+          specialize (H8 (y, L)). intuition.
+        * assert (evalid G (y, R)) by
+              (apply (@right_valid _ _ _ _ _ _ _ (biGraph G)); auto).
+          subst r. symmetry. specialize (H10 (y, R)).
+          specialize (H8 (y, R)). intuition.
   Qed.
 
-  Lemma axiom_3 : forall v G1 G2 G G3 x l r, valid (imp (and (lookup G x v l r) (and (mark G r G1) (and (neq v 1) (and (mark G1 l G2) (update G2 x 1 l r G3))))) (and (mark G x G3) (lookup G3 x 1 l r))).
+  Lemma axiom_8 : forall l r x G, valid (imp (lookup G x true l r) (mark G x G)).
   Proof.
-    intros; intro w; hnf; unfold and; hnf; intros. destruct H as [? [? [? [? ?]]]]. destruct H as [? [? [? [? ?]]]]. hnf in H1.
-    assert ((b_pg_g G) ~=~ (b_pg_g G2)). destruct H0, H2. apply (si_trans H0); auto.
-    assert (mark1 adr nat natEqDec (fun d : nat => d = 1) (b_pg_g G2) x (b_pg_g G3)). apply (update_is_mark1 l r w); auto.
-    destruct (H8 x). tauto. destruct (H8 x). rewrite <- H10. auto. split.
-    apply (mark_right_left_root _ _ _ _ _ (b_pg_g G1) (b_pg_g G2) _ _ l r); auto. hnf; simpl. rewrite H. auto.
-    apply node_is_two; auto. destruct H9 as [? [? [? ?]]]. split. hnf in H11. auto. destruct H0, H2.
-    apply (three_identity_same G G1 G2); auto.
-  Qed.
-
-  Lemma axiom_4 : forall v G1 G2 G G3 x l r, valid (imp (and (lookup G x v l r) (and (mark G l G1) (and (neq v 1) (and (mark G1 r G2) (update G2 x 1 l r G3))))) (and (mark G x G3) (lookup G3 x 1 l r))).
-  Proof.
-    intros; intro w; hnf; unfold and; hnf; intros. destruct H as [? [? [? [? ?]]]]. destruct H as [? [? [? [? ?]]]]. hnf in H1.
-    assert ((b_pg_g G) ~=~ (b_pg_g G2)). destruct H0, H2. apply (si_trans H0); auto.
-    assert (mark1 adr nat natEqDec (fun d : nat => d = 1) (b_pg_g G2) x (b_pg_g G3)). apply (update_is_mark1 l r w); auto.
-    destruct (H8 x). tauto. destruct (H8 x). rewrite <- H10. auto. split.
-    apply (mark_left_right_root _ _ _ _ _ (b_pg_g G1) (b_pg_g G2) _ _ l r); auto. hnf; simpl. rewrite H. auto.
-    apply node_is_two; auto. destruct H9 as [? [? [? ?]]]. split. hnf in H11. auto. destruct H0, H2.
-    apply (three_identity_same G G1 G2); auto.
-  Qed.
-
-  Lemma axiom_5 : forall v G1 G2 G G3 x l r, valid (imp (and (lookup G x v l r) (and (update G x 1 l r G1) (and (neq v 1) (and (mark G1 r G2) (mark G2 l G3))))) (and (mark G x G3) (lookup G3 x 1 l r))).
-  Proof.
-    intros; intro w; hnf; unfold and; hnf; intros. destruct H as [? [? [? [? ?]]]]. destruct H as [? [? [? [? ?]]]]. hnf in H1.
-    assert (mark1 adr nat natEqDec (fun d : nat => d = 1) (b_pg_g G) x (b_pg_g G1)). apply (update_is_mark1 l r w); auto.
-    split. apply (mark_root_right_left _ _ _ _ (b_pg_g G) (b_pg_g G1) (b_pg_g G2) (b_pg_g G3) x l r). hnf; simpl. rewrite H.
-    auto. apply node_is_two; auto. auto. apply H2. apply H3. destruct H8 as [? [? [? ?]]]. split. hnf in H10.
-    apply (marked_node_marked G2 l w); auto. apply (marked_node_marked G1 r w); auto. destruct H2, H3.
-    apply (three_identity_same G G1 G2); auto.
-  Qed.
-
-  Lemma axiom_6 : forall v G1 G2 G G3 x l r, valid (imp (and (lookup G x v l r) (and (update G x 1 l r G1) (and (neq v 1) (and (mark G1 l G2) (mark G2 r G3))))) (and (mark G x G3) (lookup G3 x 1 l r))).
-  Proof.
-    intros; intro w; hnf; unfold and; hnf; intros. destruct H as [? [? [? [? ?]]]]. destruct H as [? [? [? [? ?]]]]. hnf in H1.
-    assert (mark1 adr nat natEqDec (fun d : nat => d = 1) (b_pg_g G) x (b_pg_g G1)). apply (update_is_mark1 l r w); auto. split.
-    apply (mark_root_left_right _ _ _ _ (b_pg_g G) (b_pg_g G1) (b_pg_g G2) (b_pg_g G3) x l r). hnf; simpl. rewrite H. auto.
-    apply node_is_two; auto. auto. apply H2. apply H3. destruct H8 as [? [? [? ?]]]. split. hnf in H10.
-    apply (marked_node_marked G2 r w); auto. apply (marked_node_marked G1 l w); auto.
-    destruct H2 as [? _]. destruct H3 as [? _]. apply (three_identity_same G G1 G2); auto.
-  Qed.
-
-  Lemma axiom_7 : forall v G x G1 y l r, valid (imp (and (mark G x G1) (lookup G y v l r)) (and (subset_reach G x G1) (and (eq_notreach G x G1) (ext (fun Anon_15 => (lookup G1 y Anon_15 l r)))))).
-  Proof.
-    intros. intro w. unfold and. hnf. intros. destruct H. unfold mark in H. split. unfold subset_reach.
-    apply mark_reachable with (marked := fun d => d = 1). auto. split. unfold eq_notreach.
-    apply (mark_unreachable_subgraph _ _ _ (fun d => d = 1)). auto.
-
-    unfold ext. destruct H0 as [? [? [? [? ?]]]]. destruct H as [? [? ?]]. destruct (H y). hnf. unfold lookup.
-    specialize (H5 y). specialize (H6 y). LEM ((b_pg_g G) |= x ~o~> y satisfying (unmarked nat (fun d : nat => d = 1))).
-    specialize (H5 H9). hnf in H5. exists 1. split; auto. split. apply H7. auto. split. destruct (H l). apply H10. auto.
-    split. destruct (H r). apply H10; auto. rewrite <- H8. auto. specialize (H6 H9). exists v. split. rewrite <- H6. auto.
-    split. apply H7. auto. split. destruct (H l). apply H10; auto. split. destruct (H r). apply H10; auto. rewrite <- H8. auto.
-  Qed.
-
-  Lemma axiom_8 : forall l r x G, valid (imp (lookup G x 1 l r) (mark G x G)).
-  Proof.
-    intros. intro. hnf. intros. destruct H as [?[? [? [? ?]]]]. split. apply si_refl. split; intros. hnf. unfold unmarked in H4.
-    destruct H4 as [p [[? ?] [? ?]]]. unfold path_prop in H7. specialize (H7 x). assert (In x p). destruct p. simpl in H4.
-    inversion H4. simpl in H4. inversion H4. subst. apply in_eq. specialize (H7 H8). hnf in H7. exfalso; auto. auto.
+    intros. unfold valid, imp, lookup, mark. rewrite <- iter_sepcon.prop_impl_imp. normalize.
+    destruct H as [? [? [? [? [? ?]]]]]. hnf. split; [|reflexivity].
+    split; [|split]; [reflexivity | intros..]; [intuition|destruct H5; auto].
+    apply reachable_by_head_prop in H5. simpl in H5. unfold Complement in H5. unfold In in H5.
+    exfalso; auto.
   Qed.
 
   Lemma axiom_9 : forall G, valid (mark G null_node G).
   Proof.
-    intros. intro w. unfold null_node. split; clear w. apply si_refl. split; intros. hnf. unfold unmarked in H.
-    destruct H as [p [[? ?] [? ?]]]. destruct p. inversion H. simpl in H. inversion H. subst. simpl in H1. destruct p.
-    unfold b_pg_g in H1. rewrite <- pg_the_same in H1. apply valid_not_null in H1. exfalso; auto. destruct H1 as [[? _] _].
-    unfold b_pg_g in H1. rewrite <- pg_the_same in H1. apply valid_not_null in H1. exfalso; auto. auto.
+    intros. unfold valid, mark, null_node. normalize. hnf. split; [|reflexivity].
+    hnf. split; [|intros; split; intros]; [reflexivity | intuition |]. destruct H; auto.
+    exfalso. apply reachable_by_head_valid in H.
+    apply (@valid_not_null _ _ _ _ _ (maGraph G) _) in H; auto. rewrite is_null_def. auto.
   Qed.
 
-  Lemma lookup_graph_unfold: forall G v x l r w,
-                               lookup G x v l r w -> (graph x G = trinode x v l r ⊗ graph l G ⊗ graph r G)%pred.
+  Lemma lookup_graph_unfold: forall (G: A) x v l r,
+      vlabel G x = v -> vvalid G x -> vvalid G l -> vvalid G r -> dst G (x, L) = l ->
+      dst G (x, R) = r -> (graph x G = ptto_node x v l r ⊗ graph l G ⊗ graph r G).
   Proof.
-    intros. destruct H as [? [? [? [? ?]]]]. clear w. apply pred_ext; intro w; intro. rewrite graph_unfold in H4.
-    destruct H4 as [[? ?] | [dd [ll [rr [[? ?] ?]]]]]. hnf in H4. unfold b_pg_g in H0. rewrite <- pg_the_same in H0.
-    apply valid_not_null in H0. exfalso; auto. unfold gamma in H4. unfold biEdge in H4.
-    destruct (@only_two_neighbours adr nat natEqDec (@bm_bi adr nat O natEqDec G) x) as [v1 [v2 ?]] in H4. unfold b_pg_g in H3.
-    rewrite H3 in e. inversion e. subst. inversion H4. subst. apply H6. rewrite graph_unfold. right. exists v, l, r. split.
-    split. unfold gamma, biEdge. destruct (@only_two_neighbours adr nat natEqDec (@bm_bi adr nat O natEqDec G)x) as [v1 [v2 ?]].
-    unfold b_pg_g in H3. rewrite H3 in e. inversion e. subst. auto. auto. auto.
+    intros. unfold graph. unfold ptto_node. apply bi_graph_unfold; auto.
+    simpl. unfold gamma. f_equal; [f_equal|]; auto.
   Qed.
 
   Lemma graph_graphs_eq_l:
-    forall G v x l r w, lookup G x v l r w ->
-                        (trinode x v l r ⊗ (graph l G ⊗ graph r G) = graph l G ⊗ graphs (x :: l :: r :: nil) G)%pred.
+    forall (G: A) v x l r, vlabel G x = v -> vvalid G x -> vvalid G l -> vvalid G r ->
+                           dst G (x, L) = l -> dst G (x, R) = r ->
+                           (ptto_node x v l r ⊗ (graph l G ⊗ graph r G)) =
+                           graph l G ⊗ graphs (x :: l :: r :: nil)
+                                 (GraphBi.Graph_SpatialGraph G).
   Proof.
-    intros. apply lookup_graph_unfold in H. rewrite <- ocon_assoc. unfold graphs. rewrite ocon_emp. do 2 rewrite <- ocon_assoc.
-    rewrite (ocon_comm (graph l G) (graph x G)). rewrite (ocon_assoc (graph x G) (graph l G) (graph l G)).
-    rewrite ocon_precise_elim. rewrite (ocon_assoc (graph x G) (graph l G) (graph r G)). rewrite H.
-    rewrite (ocon_assoc (trinode x v l r) (graph l G) (graph r G)).
-    rewrite (ocon_assoc (trinode x v l r) (graph l G ⊗ graph r G) (graph l G ⊗ graph r G)). rewrite ocon_precise_elim. auto.
-    apply precise_ocon; apply precise_graph. apply precise_graph.
+    intros. simpl. rewrite ocon_emp. do 3 rewrite <- ocon_assoc.
+    rewrite (ocon_comm (graph l G) (graph x G)).
+    rewrite (ocon_assoc (graph x G) (graph l G) (graph l G)).
+    rewrite <- log_normalize.precise_ocon_self.
+    2: apply (bi_graph_precise_left _ x); auto.
+    rewrite (lookup_graph_unfold _ x v l r); auto.
+    rewrite (ocon_assoc (ptto_node x v l r) (graph l G) (graph r G)).
+    rewrite ocon_assoc.
+    rewrite (ocon_assoc (ptto_node x v l r) (graph l G ⊗ graph r G)
+                        (graph l G ⊗ graph r G)).
+    rewrite <- log_normalize.precise_ocon_self; auto. apply precise_ocon.
+    + apply (bi_graph_precise_left _ x); auto.
+    + apply (bi_graph_precise_right _ x); auto.
   Qed.
 
-  Lemma lem_subgraphupdate_l : forall G v G1 x v1 l r, valid (imp (and (star (graph l G1) (mwand (graph l G) (union (ptto_node x v l r) (union (graph l G) (graph r G))))) (and (subset_reach G l G1) (and (eq_notreach G l G1) (and (lookup G x v l r) (lookup G1 x v1 l r))))) (union (ptto_node x v1 l r) (union (graph l G1) (graph r G1)))).
+  Lemma lem_subgraphupdate_l : forall G v G1 x v1 l r,
+      valid (imp (and (star (graph l G1) (mwand (graph l G) (union (ptto_node x v l r) (union (graph l G) (graph r G)))))
+                      (and (subset_reach G l G1) (and (eq_notreach G l G1) (and (lookup G x v l r) (lookup G1 x v1 l r)))))
+                 (union (ptto_node x v1 l r) (union (graph l G1) (graph r G1)))).
   Proof.
-    intros. intro w; hnf. unfold and, star, union, mwand, subset_reach, eq_notreach, ptto_node. intros.
-    destruct H as [? [? [? [? ?]]]].
-    assert (subset (reachable_through_set (b_pg_g G) (l :: nil)) (reachable_through_set (b_pg_g G1) (l :: nil))).
-    unfold reachable_through_set. intro n; intros. destruct H4 as [s [? ?]]; exists s. split; auto. apply in_inv in H4.
-    destruct H4. subst. apply H0; auto. inversion H4. clear H0.
-    generalize (subgraph_update_ewand G G1 (l :: nil) (l :: nil) (x :: l :: r :: nil) H4 H1). intro.
-    unfold graphs in H0 at 1 2 3 5. do 2 rewrite ocon_emp in H0. apply graph_graphs_eq_l in H2. rewrite H2 in H.
-    specialize (H0 w H).  apply graph_graphs_eq_l in H3. rewrite H3. auto.
-  Qed.
+    intros. unfold valid, imp, and, star, graph, mwand, union, subset_reach, eq_notreach, ptto_node.
+  Admitted.
+  
+  Lemma axiom_1 : forall v G1 G2 G G3 x l r, valid (imp (and (lookup G x v l r) (and (mark G r G1) (and (neq v true) (and (mark G2 l G3) (update G1 x true l r G2))))) (and (mark G x G3) (lookup G3 x true l r))).
+  Proof.
+  Admitted.
 
-  Lemma graph_graphs_eq_r:
+  Lemma axiom_2 : forall v G1 G2 G G3 x l r, valid (imp (and (lookup G x v l r) (and (mark G l G1) (and (neq v true) (and (mark G2 r G3) (update G1 x true l r G2))))) (and (mark G x G3) (lookup G3 x true l r))).
+  Proof.
+  Admitted.
+
+  Lemma axiom_3 : forall v G1 G2 G G3 x l r, valid (imp (and (lookup G x v l r) (and (mark G r G1) (and (neq v true) (and (mark G1 l G2) (update G2 x true l r G3))))) (and (mark G x G3) (lookup G3 x true l r))).
+  Proof.
+  Admitted.
+
+  Lemma axiom_4 : forall v G1 G2 G G3 x l r, valid (imp (and (lookup G x v l r) (and (mark G l G1) (and (neq v true) (and (mark G1 r G2) (update G2 x true l r G3))))) (and (mark G x G3) (lookup G3 x true l r))).
+  Proof.
+  Admitted.
+
+  Lemma axiom_5 : forall v G1 G2 G G3 x l r, valid (imp (and (lookup G x v l r) (and (update G x true l r G1) (and (neq v true) (and (mark G1 r G2) (mark G2 l G3))))) (and (mark G x G3) (lookup G3 x true l r))).
+  Proof.
+  Admitted.
+
+  (* Lemma graph_graphs_eq_r:
     forall G v x l r w, lookup G x v l r w ->
-                        (trinode x v l r ⊗ (graph l G ⊗ graph r G) = graph r G ⊗ graphs (x :: l :: r :: nil) G)%pred.
+                        (ptto_node x v l r ⊗ (graph l G ⊗ graph r G) = graph r G ⊗ graphs (x :: l :: r :: nil) G)%pred.
   Proof.
     intros. apply lookup_graph_unfold in H. rewrite <- ocon_assoc. unfold graphs. rewrite ocon_emp. do 2 rewrite <- ocon_assoc.
     rewrite (ocon_comm (graph r G) (graph x G)). rewrite H. rewrite (ocon_assoc (trinode x v l r ⊗ graph l G)).
@@ -238,31 +258,14 @@ Module GraphMark <: Mgraphmark.
     rewrite (ocon_assoc (trinode x v l r ⊗ (graph l G ⊗ graph r G))).
     rewrite (ocon_assoc (trinode x v l r) (graph l G ⊗ graph r G) (graph l G ⊗ graph r G)). rewrite ocon_precise_elim.
     rewrite ocon_assoc. auto. apply precise_ocon; apply precise_graph. apply precise_graph.
-  Qed.
+  Qed. *)
 
   Lemma lem_subgraphupdate_r : forall G v G1 x v1 l r, valid (imp (and (star (graph r G1) (mwand (graph r G) (union (ptto_node x v l r) (union (graph l G) (graph r G))))) (and (subset_reach G r G1) (and (eq_notreach G r G1) (and (lookup G x v l r) (lookup G1 x v1 l r))))) (union (ptto_node x v1 l r) (union (graph l G1) (graph r G1)))).
   Proof.
-    intros. intro w; hnf. unfold and, star, union, mwand, subset_reach, eq_notreach, ptto_node. intros.
-    destruct H as [? [? [? [? ?]]]].
-    assert (subset (reachable_through_set (b_pg_g G) (r :: nil)) (reachable_through_set (b_pg_g G1) (r :: nil))).
-    unfold reachable_through_set. intro n; intros. destruct H4 as [s [? ?]]; exists s. split; auto. apply in_inv in H4.
-    destruct H4. subst. apply H0; auto. inversion H4. clear H0.
-    generalize (subgraph_update_ewand G G1 (r :: nil) (r :: nil) (x :: l :: r :: nil) H4 H1). intro.
-    unfold graphs in H0 at 1 2 3 5. do 2 rewrite ocon_emp in H0. apply graph_graphs_eq_r in H2. rewrite H2 in H.
-    specialize (H0 w H).  apply graph_graphs_eq_r in H3. rewrite H3. auto.
-  Qed.
+  Admitted.
 
   Lemma lem_pttoupdate : forall v G x v1 l r G1, valid (imp (and (star (ptto_node x v1 l r) (mwand (ptto_node x v l r) (union (ptto_node x v l r) (union (graph l G) (graph r G))))) (and (lookup G x v l r) (update G x v1 l r G1))) (union (ptto_node x v1 l r) (union (graph l G1) (graph r G1)))).
   Proof.
-    intros. intro w; hnf. unfold and, star, union, mwand, subset_reach, eq_notreach, ptto_node. intros.
-    destruct H as [? [? ?]]. generalize (lookup_graph_unfold _ _ _ _ _ _ H0); intro. destruct H1 as [Hn [Hi ?]].
-    apply eq_sym in H1. rewrite ocon_assoc in H2. rewrite <- H2 in H. destruct H0 as [? [? [? [? ?]]]].
-    assert (@gamma adr nat natEqDec (@bm_bi adr nat O natEqDec G) x = (v, l, r)). unfold gamma, biEdge.
-    destruct (@only_two_neighbours adr nat natEqDec (@bm_bi adr nat O natEqDec G) x) as [t1 [t2 ?]]. unfold b_pg_g in H6.
-    rewrite H6 in e. inversion e; subst. auto. generalize (single_graph_node_update_2_ewand G x v l r v1 G1 Hn Hi H7 H1 w H).
-    intro. assert (lookup G1 x v1 l r w). subst. split; simpl. unfold change_node_label. destruct (@t_eq_dec adr natEqDec x x).
-    auto. exfalso; auto. unfold change_valid. do 3 (split;auto). unfold change_edge_func. destruct (@t_eq_dec adr natEqDec x x).
-    auto. exfalso; auto. apply lookup_graph_unfold in H9. rewrite <- ocon_assoc. rewrite <- H9. apply H8.
-  Qed.
+  Admitted.
 
 End GraphMark.
